big refactor to use new dafny language features and simplify verification
 * introduce new subset types for word and mem; use them to clean up a
   lot of defs (mainly isUInt32 and WordAligned predicates)

 * delete assembly.s.dfy; use new bitvector support to reason about
   bitwise ops directly

 * remove duplicate/trivial abstractions to help with
   reasoning/triggering: ValidDestinationOperand, AlwaysInvariant,
   op_*(), eval_op, addrval, addr_mem

 * make ValidMem and ValidMemRange independent of the state

verification status:
 * bitvector math still requires axioms/assumes
 * allocate_page: 1 timeout
 * init_l2ptable: 1 error
 * enter_resume: Spartan crash

overall better than before, but we still see timeouts/failures in *.sdfy

verified/ARMdef.dfy
@@ -1,12 +1,23 @@
-include "assembly.s.dfy"
 include "Maybe.dfy"
 include "Seq.dfy"
+
+//-----------------------------------------------------------------------------
+// Core types (for a 32-bit word-aligned machine)
+//-----------------------------------------------------------------------------
+predicate isUInt32(i:int) { 0 <= i < 0x1_0000_0000 }
+function BytesPerWord() : int { 4 }
+predicate WordAligned(i:int) { i % 4 == 0 }
+function WordsToBytes(w:int) : int { 4 * w }
+function BytesToWords(b:int) : int requires WordAligned(b) { b / 4 }
+
+type word = x | isUInt32(x)
+type mem = x | isUInt32(x) && WordAligned(x) // TODO: would be better named "addr"
 
 //-----------------------------------------------------------------------------
 // Microarchitectural State
 //-----------------------------------------------------------------------------
 // NB: In FIQ mode, R8 to R12 are also banked, but we don't model this
-datatype ARMReg = R0|R1|R2|R3|R4|R5|R6|R7|R8|R9|R10|R11|R12 | SP(spm:mode) | LR(lrm:mode)
+datatype ARMReg = R0|R1|R2|R3|R4|R5|R6|R7|R8|R9|R10|R11|R12| SP(spm:mode) | LR(lrm:mode)
 
 // Special register instruction operands
 datatype SReg = cpsr | spsr(m:mode) | scr | ttbr0
@@ -23,18 +34,18 @@ datatype PSR  = PSR(m:mode)           // See B1.3.3
 datatype SCR  = SCR(ns:world, irq:bool, fiq:bool) // See B4.1.129
 datatype TTBR = TTBR(ptbase:mem)      // See B4.1.154
 
-type mem = int
-datatype operand = OConst(n:int) 
-    | OReg(r:ARMReg) 
+datatype operand = OConst(n:word)
+    | OReg(r:ARMReg)
     | OSymbol(sym:string)
     | OSReg(sr:SReg)
-    | OSP | OLR 
+    | OSP | OLR
 
-datatype memstate = MemState(addresses:map<mem, int>,
-                             globals:map<operand, seq<int>>)
+type memmap = map<mem, word>
+datatype memstate = MemState(addresses:memmap,
+                             globals:map<operand, seq<word>>)
 
-datatype state = State(regs:map<ARMReg, int>,
-                       sregs:map<SReg, int>,
+datatype state = State(regs:map<ARMReg, word>,
+                       sregs:map<SReg, word>,
                        m:memstate,
                        conf:config,
                        ok:bool,
@@ -45,24 +56,6 @@ datatype mode = User | FIQ | IRQ | Supervisor | Abort | Undefined | Monitor
 datatype priv = PL0 | PL1 // PL2 is only used in Hyp, not modeled
 datatype world = Secure | NotSecure
 datatype exception = ExAbt | ExUnd | ExIRQ | ExFIQ | ExSVC
-
-//-----------------------------------------------------------------------------
-// TODO: get rid of these.
-//-----------------------------------------------------------------------------
-function method op_r(r:ARMReg):operand
-    { OReg(r) }
-
-function method op_sp():operand
-    { OSP }
-
-function method op_lr():operand
-    { OLR }
-
-function method op_sym(sym:string):operand
-    { OSymbol(sym) }
-
-function op_spsr(s:state):operand
-    { OSReg(spsr(mode_of_state(s))) }
 
 //-----------------------------------------------------------------------------
 // Configuration State
@@ -94,34 +87,35 @@ function priv_of_state(s:state):priv
 
 // In real life these are more complicated. Add more as needed!
 
+function psr_mask_mode(v:word): word
+{
+    BitwiseAnd(v, 0x1f)
+}
+
 // See B1.3.3
-function decode_psr(v:int) : PSR
-    requires isUInt32(v)
-    requires ValidModeEncoding(and32(v,0x1f))
-    { PSR(decode_mode(and32(v, 0x1f))) }
+function decode_psr(v:word) : PSR
+    requires ValidModeEncoding(psr_mask_mode(v))
+    { PSR(decode_mode(psr_mask_mode(v))) }
 
 // See B4.1.129
-function decode_scr(v:int) : SCR
-    requires isUInt32(v)
+function decode_scr(v:word) : SCR
 {
     SCR(
-        if and32(v, 1) != 0 then NotSecure else Secure,
-        and32(v, 2) != 0, // IRQ bit
-        and32(v, 4) != 0 // FIQ bit
+        if BitwiseAnd(v, 1) != 0 then NotSecure else Secure,
+        BitwiseAnd(v, 2) != 0, // IRQ bit
+        BitwiseAnd(v, 4) != 0 // FIQ bit
         )
 }
 
-function decode_ttbr(v:int): TTBR
-    requires isUInt32(v)
+function decode_ttbr(v:word): TTBR
     ensures PageAligned(decode_ttbr(v).ptbase)
     // assuming 4k alignment, n == 2 / x == 12
-    { MaskWithSizeIsAligned(v, 0x1000); TTBR(and32(v, 0xffff_f000)) }
+    { MaskWithSizeIsAligned(v, 0x1000); TTBR(BitwiseAnd(v, 0xffff_f000)) }
 
-function decode_sreg(s:state, sr:SReg, v:int) : config
+function decode_sreg(s:state, sr:SReg, v:word): config
     requires ValidConfig(s.conf)
     requires ValidSpecialOperand(s, OSReg(sr))
-    requires isUInt32(v)
-    requires (sr.cpsr? || sr.spsr?) ==> ValidModeEncoding(and32(v, 0x1f))
+    requires (sr.cpsr? || sr.spsr?) ==> ValidModeEncoding(psr_mask_mode(v))
     ensures ValidConfig(decode_sreg(s, sr, v))
 {
     // reveal_ValidConfig();
@@ -138,10 +132,10 @@ function decode_sreg(s:state, sr:SReg, v:int) : config
 //-----------------------------------------------------------------------------
 // Mode / Security State Decoding / Encoding
 //-----------------------------------------------------------------------------
-function method encode_ns(ns:world):int
+function method encode_ns(ns:world): word
     { if ns == NotSecure then 1 else 0 }
 
-function method encode_mode(m:mode):int
+function method encode_mode(m:mode): word
 {
     match m
         case User => 0x10
@@ -153,7 +147,7 @@ function method encode_mode(m:mode):int
         case Monitor => 0x16
 }
 
-function method decode_mode'(e:int):Maybe<mode>
+function method decode_mode'(e:word):Maybe<mode>
 {
     if e == 0x10 then Just(User)
     else if e == 0x11 then Just(FIQ)
@@ -170,12 +164,12 @@ lemma mode_encodings_are_sane()
     ensures forall m :: decode_mode'(encode_mode(m)) == Just(m)
 {}
 
-predicate ValidModeEncoding(e:int)
+predicate ValidModeEncoding(e:word)
 {
     decode_mode'(e).Just?
 }
 
-function method decode_mode(e:int):mode
+function method decode_mode(e:word):mode
     requires ValidModeEncoding(e)
 {
     fromJust(decode_mode'(e))
@@ -192,7 +186,6 @@ datatype ins =
     | AND(dstAND:operand, src1AND:operand, src2AND:operand)
     | ORR(dstOR:operand,  src1OR:operand,  src2OR:operand)
     | EOR(dstEOR:operand, src1EOR:operand, src2EOR:operand) // Also known as XOR
-    | ROR(dstROR:operand, src1ROR:operand, src2ROR:operand)
     | LSL(dstLSL:operand, src1LSL:operand, src2LSL:operand)
     | LSR(dstLSR:operand, src1LSR:operand, src2LSR:operand)
     | MOV(dstMOV:operand, srcMOV:operand)
@@ -231,27 +224,6 @@ datatype code =
 | While(whileCond:obool, whileBody:code)
 
 //-----------------------------------------------------------------------------
-// Microarch-Related Utilities
-//-----------------------------------------------------------------------------
-predicate isUInt32(i:int) { 0 <= i < 0x1_0000_0000 }
-function BytesPerWord() : int { 4 }
-predicate WordAligned(addr:int) { addr % 4 == 0}
-function WordsToBytes(w:int) : int { 4 * w }
-function BytesToWords(b:int) : int requires WordAligned(b) { b / 4 }
-
-// FIXME: delete or move elsewhere
-lemma WordAlignedAdd(x1:int,x2:int)
-    requires WordAligned(x1) && WordAligned(x2)
-    ensures  WordAligned(x1+x2)
-    {}
-
-// FIXME: delete or move elsewhere
-lemma WordAlignedAdd_(x1:int,x2:int,y:int)
-    requires WordAligned(x1) && WordAligned(x2) && y == x1+x2
-    ensures WordAligned(y)
-    {}
-
-//-----------------------------------------------------------------------------
 // Validity
 //-----------------------------------------------------------------------------
 predicate ValidState(s:state)
@@ -260,69 +232,44 @@ predicate ValidState(s:state)
     ValidConfig(s.conf) && ValidSRegState(s.sregs)
 }
 
-predicate {:opaque} ValidRegState(regs:map<ARMReg, int>)
+predicate {:opaque} ValidRegState(regs:map<ARMReg, word>)
 {
-    (forall m:mode {:trigger SP(m)} {:trigger LR(m)} ::
-        SP(m) in regs && isUInt32(regs[SP(m)]) &&
-        LR(m) in regs && isUInt32(regs[LR(m)]))
-    && R0 in regs && isUInt32(regs[R0])
-    && R1 in regs && isUInt32(regs[R1])
-    && R2 in regs && isUInt32(regs[R2])
-    && R3 in regs && isUInt32(regs[R3])
-    && R4 in regs && isUInt32(regs[R4])
-    && R5 in regs && isUInt32(regs[R5])
-    && R6 in regs && isUInt32(regs[R6])
-    && R7 in regs && isUInt32(regs[R7])
-    && R8 in regs && isUInt32(regs[R8])
-    && R9 in regs && isUInt32(regs[R9])
-    && R10 in regs && isUInt32(regs[R10])
-    && R11 in regs && isUInt32(regs[R11])
-    && R12 in regs && isUInt32(regs[R12])
+    forall r:ARMReg :: r in regs
 }
 
 predicate ValidConfig(c:config)
 {
-    isUInt32(c.ttbr0.ptbase) && PageAligned(c.ttbr0.ptbase) &&
-    User !in c.spsr &&
+    PageAligned(c.ttbr0.ptbase) && User !in c.spsr &&
     (forall m:mode :: m != User ==> m in c.spsr )
 }
 
-predicate {:opaque} ValidSRegState(sregs:map<SReg, int>)
+predicate {:opaque} ValidSRegState(sregs:map<SReg, word>)
 {
-    (forall m:mode {:trigger spsr(m)} :: m != User ==> 
-        spsr(m) in sregs && isUInt32(sregs[spsr(m)]))
+    (forall m:mode {:trigger spsr(m)} :: m != User ==> spsr(m) in sregs)
     && spsr(User) !in sregs
-    && ttbr0 in sregs && isUInt32(sregs[ttbr0])
-    && scr   in sregs && isUInt32(sregs[scr])
-    && cpsr  in sregs && isUInt32(sregs[cpsr])
-    && ValidModeEncoding(and32(sregs[cpsr], 0x1f))
+    && ttbr0 in sregs && scr in sregs && cpsr in sregs
+    && ValidModeEncoding(psr_mask_mode(sregs[cpsr]))
 }
 
 // All valid states have the same memory address domain, but we don't care what 
 // it is (at this level).
-function {:axiom} AddressDomain() : set<mem>
+function {:axiom} TheValidAddresses() : set<mem>
+    ensures forall m :: m in TheValidAddresses() ==> WordAligned(m)
 
 predicate {:opaque} ValidMemState(s:memstate)
 {
     // regular mem
-    (forall m:mem :: m in AddressDomain() <==> m in s.addresses)
-    && (forall m:mem :: m in s.addresses
-        ==> WordAligned(m) && isUInt32(m) && isUInt32(s.addresses[m]))
-    // globals
-    && (match TheGlobalDecls() case GlobalDecls(decls) =>
-        // same names as decls
-        // The parentheses on the following line do actually matter!
-        (forall g :: g in decls ==> g in s.globals)
-        // correct size, all uint32 values
-        && forall g :: g in s.globals ==> (g in decls
-            && WordsToBytes(|s.globals[g]|) == decls[g]
-            && forall v :: v in s.globals[g] ==> isUInt32(v)))
+    (forall m:mem :: m in TheValidAddresses() <==> m in s.addresses)
+    // globals: same names/sizes as decls
+    && (forall g :: g in TheGlobalDecls() <==> g in s.globals)
+    && (forall g :: g in TheGlobalDecls()
+        ==> |s.globals[g]| == BytesToWords(TheGlobalDecls()[g]))
 }
 
 predicate ValidOperand(o:operand)
 {
     match o
-        case OConst(n) => isUInt32(n)
+        case OConst(n) => true
         case OReg(r) => !(r.SP? || r.LR?) // not used directly
         case OSP => true
         case OLR => true
@@ -333,8 +280,7 @@ predicate ValidOperand(o:operand)
 predicate ValidSpecialOperand(s:state, o:operand)
 {
     o.OSReg? && ValidConfig(s.conf) && mode_of_state(s) != User
-    &&(
-        (o.sr.spsr? && mode_of_state(s) == o.sr.m)
+    &&( (o.sr.spsr? && mode_of_state(s) == o.sr.m)
      || (o.sr.scr?  && world_of_state(s) == Secure)
      || (!o.sr.spsr? && !o.sr.scr?))
 }
@@ -344,61 +290,52 @@ predicate ValidMcrMrcOperand(s:state,o:operand)
     ValidSpecialOperand(s,o) && o.sr.scr?
 }
 
-predicate ValidMem(s:memstate, m:mem)
+predicate ValidMem(addr:int)
 {
-    isUInt32(m) && WordAligned(m) && m in s.addresses
+    isUInt32(addr) && WordAligned(addr) && addr in TheValidAddresses()
 }
 
-predicate ValidMemRange(s:memstate, base:int, limit:int)
+predicate ValidMemRange(base:int, limit:int)
 {
-    forall i:int :: base <= i < limit && WordAligned(i) ==>
-        ValidMem(s, i)
+    isUInt32(base) && isUInt32(limit) &&
+    forall m:mem :: base <= m < limit && WordAligned(m) ==> m in TheValidAddresses()
 }
 
 predicate ValidShiftOperand(s:state, o:operand)
     requires ValidState(s)
     { ValidOperand(o) && OperandContents(s, o) < 32 }
 
-predicate ValidDestinationOperand(o:operand)
-    { !o.OConst? && ValidOperand(o) }
-
-// MUL only operates on regs
-// Currently the same as ValidDestinationOperand, but in the future globals
-// might be valid destinations but not registers. 
 predicate ValidRegOperand(o:operand)
     { !o.OConst? && ValidOperand(o) }
 
 //-----------------------------------------------------------------------------
 // Globals
 //-----------------------------------------------------------------------------
-datatype globaldecls = GlobalDecls(map<operand, int>)
+type globaldecls = map<operand, word>
 
 predicate ValidGlobal(o:operand)
 {
-    match TheGlobalDecls() case GlobalDecls(declmap) =>
-        o.OSymbol? && o in declmap
+    o.OSymbol? && o in TheGlobalDecls()
 }
 
-predicate ValidGlobalDecls(gd:globaldecls)
+predicate ValidGlobalDecls(decls:globaldecls)
 {
-    gd.GlobalDecls? && match gd case GlobalDecls(decls) =>
-        forall d :: d in decls ==> d.OSymbol? && decls[d] > 0 && WordAligned(decls[d])
+    forall d :: d in decls ==> d.OSymbol? && decls[d] > 0 && WordAligned(decls[d])
 }
 
-predicate ValidGlobalOffset(g:operand, offset:int)
+predicate ValidGlobalOffset(g:operand, offset:word)
 {
     ValidGlobal(g) && WordAligned(offset) && 0 <= offset < SizeOfGlobal(g)
 }
 
 // globals have an unknown (uint32) address, only establised by LDR-reloc
-function {:axiom} AddressOfGlobal(g:operand): int
-    ensures isUInt32(AddressOfGlobal(g));
+function {:axiom} AddressOfGlobal(g:operand): mem
 
-function SizeOfGlobal(g:operand): int
+function SizeOfGlobal(g:operand): word
     requires ValidGlobal(g)
     ensures WordAligned(SizeOfGlobal(g))
 {
-    match TheGlobalDecls() case GlobalDecls(declmap) => declmap[g]
+    TheGlobalDecls()[g]
 }
 
 // global declarations are the responsibility of the program, as long as they're valid
@@ -421,7 +358,6 @@ function mode_of_exception(conf:config, e:exception): mode
 predicate evalExceptionTaken(s:state, e:exception, r:state)
     requires ValidState(s)
     ensures evalExceptionTaken(s, e, r) ==> ValidState(r)
-    // ensures evalExceptionTaken(s, e, r) ==> AlwaysInvariant(s, r)
 {
     reveal_ValidRegState();
     // reveal_ValidConfig();
@@ -429,7 +365,7 @@ predicate evalExceptionTaken(s:state, e:exception, r:state)
     var oldmode := mode_of_state(s);
     var newmode := mode_of_exception(s.conf, e);
     // this does not model all of the CPSR update, since we don't model all the bits
-    var newpsr := or32(and32(s.sregs[cpsr], 0xffffffe0), encode_mode(newmode));
+    var newpsr := BitwiseOr(BitwiseAnd(s.sregs[cpsr], 0xffffffe0), encode_mode(newmode));
     ValidState(r) &&
     // update mode, copy CPSR of oldmode to SPSR of newmode, havoc LR
     r == s.(conf := s.conf.(cpsr := PSR(newmode),
@@ -449,9 +385,9 @@ predicate evalEnterUserspace(s:state, r:state)
     ensures evalEnterUserspace(s, r) ==> mode_of_state(r) == User
 {
     mode_of_state(s) != User && ValidModeChange'(s, User) &&
-    var spsr := op_spsr(s);
+    var spsr := OSReg(spsr(mode_of_state(s)));
     assert ValidSpecialOperand(s, spsr);
-    decode_mode'(and32(SpecialOperandContents(s, spsr), 0x1f)) == Just(User) &&
+    decode_mode'(psr_mask_mode(SpecialOperandContents(s, spsr))) == Just(User) &&
     evalSRegUpdate(s, OSReg(cpsr), SpecialOperandContents(s,spsr), r)
 }
 
@@ -477,11 +413,10 @@ predicate evalUserspaceExecution(s:state, r:state)
         ==> r.regs[SP(m)] == s.regs[SP(m)] && r.regs[LR(m)] == s.regs[LR(m)])
 }
 
-function havocPages(pages:set<mem>, s:map<mem, int>, r:map<mem, int>): map<mem, int>
+function havocPages(pages:set<mem>, s:memmap, r:memmap): memmap
     requires forall m :: m in s <==> m in r
 {
-    (map m | isUInt32(m) && m in s
-        :: if and32(m, 0xffff_f000) in pages then r[m] else s[m])
+    (map m | m in s :: if BitwiseAnd(m, 0xffff_f000) in pages then r[m] else s[m])
 }
 
 // XXX: To be defined by application code
@@ -496,7 +431,7 @@ predicate ApplicationUsermodeContinuationInvariant(s:state, r:state)
 
 function method PAGESIZE():int { 0x1000 }
 
-predicate PageAligned(addr:mem)
+predicate PageAligned(addr:int)
     ensures PageAligned(addr) ==> WordAligned(addr)
 {
     // FIXME: help out poor dafny
@@ -534,7 +469,7 @@ predicate WellformedAbsL2PTable(pt: AbsL2PTable)
 
 predicate WellformedAbsPTE(pte: AbsPTE)
 {
-    PageAligned(pte.phys)
+    PageAligned(pte.phys) && isUInt32(pte.phys + PhysBase())
 }
 
 function ExtractAbsPageTable(s:state): Maybe<AbsPTable>
@@ -543,8 +478,8 @@ function ExtractAbsPageTable(s:state): Maybe<AbsPTable>
         r.Just? ==> WellformedAbsPTable(fromJust(r))
 {
     // reveal_ValidConfig();
-    var vbase := s.conf.ttbr0.ptbase + PhysBase();
-    if ValidMemRange(s.m, vbase, vbase + ARM_L1PTABLE_BYTES()) then
+    var vbase:int := s.conf.ttbr0.ptbase + PhysBase();
+    if ValidMemRange(vbase, vbase + ARM_L1PTABLE_BYTES()) then
         ExtractAbsL1PTable(s.m, vbase, 0)
     else
         Nothing
@@ -552,7 +487,7 @@ function ExtractAbsPageTable(s:state): Maybe<AbsPTable>
 
 function WritablePagesInTable(pt:AbsPTable): set<mem>
     requires WellformedAbsPTable(pt)
-    ensures forall m :: m in WritablePagesInTable(pt) ==> PageAligned(m)
+    ensures forall m:mem :: m in WritablePagesInTable(pt) ==> PageAligned(m)
 {
     (set i, j | 0 <= i < |pt| && pt[i].Just? && 0 <= j < |fromJust(pt[i])|
         && fromJust(pt[i])[j].Just? && fromJust(fromJust(pt[i])[j]).write
@@ -562,7 +497,7 @@ function WritablePagesInTable(pt:AbsPTable): set<mem>
 function ExtractAbsL1PTable(m:memstate, vbase:mem, index:nat): Maybe<AbsPTable>
     requires ValidMemState(m)
     requires WordAligned(vbase)
-        && ValidMemRange(m, vbase, vbase + ARM_L1PTABLE_BYTES())
+        && ValidMemRange(vbase, vbase + ARM_L1PTABLE_BYTES())
     requires 0 <= index <= ARM_L1PTES()
     ensures var r := ExtractAbsL1PTable(m, vbase, index);
         r.Just? ==> |fromJust(r)| == ARM_L1PTES() - index
@@ -573,7 +508,8 @@ function ExtractAbsL1PTable(m:memstate, vbase:mem, index:nat): Maybe<AbsPTable>
     // stopping condition
     if index == ARM_L1PTES() then Just([]) else
     // extract L1 PTE and check its validity
-    var pte' := ExtractAbsL1PTE(MemContents(m, vbase + index * BytesPerWord()));
+    var pte' := ExtractAbsL1PTE(
+            MemContents(m, vbase + index * BytesPerWord()));
     if pte'.Nothing? then Nothing else
     var pte := fromJust(pte');
     // extract the rest (recursive step)
@@ -584,7 +520,7 @@ function ExtractAbsL1PTable(m:memstate, vbase:mem, index:nat): Maybe<AbsPTable>
     else
         // check validity of mem pointed to by L1 PTE
         var l2vbase := fromJust(pte) + PhysBase();
-        if !ValidMemRange(m, l2vbase, l2vbase + ARM_L2PTABLE_BYTES()) then Nothing
+        if !ValidMemRange(l2vbase, l2vbase + ARM_L2PTABLE_BYTES()) then Nothing
         else
             // extract L2 table that it points to, and check its validity
             var l2table := ExtractAbsL2PTable(m, l2vbase, 0);
@@ -593,17 +529,16 @@ function ExtractAbsL1PTable(m:memstate, vbase:mem, index:nat): Maybe<AbsPTable>
 }
 
 /* ARM ref B3.5.1 short descriptor format for first-level page table */
-function ExtractAbsL1PTE(pte:int): Maybe<Maybe<int>>
-    requires isUInt32(pte)
+function ExtractAbsL1PTE(pte:word): Maybe<Maybe<mem>>
     ensures var r := ExtractAbsL1PTE(pte);
         r.Just? && fromJust(r).Just? ==> WordAligned(fromJust(fromJust(r)))
 {
     // for now, we just consider secure L1 tables in domain zero
     // (i.e., no other bits set)
-    var typebits := and32(pte, 0x3);
-    var lowbits := and32(pte, 0x3ff);
+    var typebits := BitwiseAnd(pte, 0x3);
+    var lowbits := BitwiseAnd(pte, 0x3ff);
     MaskWithSizeIsAligned(pte, 0x400);
-    var ptbase := and32(pte, 0xfffffc00);
+    var ptbase := BitwiseAnd(pte, 0xfffffc00);
     // if the type is zero, it's an invalid entry, which is fine (maps nothing)
     if typebits == 0 then Just(Nothing)
     // otherwise, the lowbits must be 1 (it maps a page table)
@@ -612,10 +547,10 @@ function ExtractAbsL1PTE(pte:int): Maybe<Maybe<int>>
     else Nothing
 }
 
-function ExtractAbsL2PTable(m:memstate, vbase:int, index:nat): Maybe<AbsL2PTable>
+function ExtractAbsL2PTable(m:memstate, vbase:mem, index:nat): Maybe<AbsL2PTable>
     requires ValidMemState(m)
     requires WordAligned(vbase)
-        && ValidMemRange(m, vbase, vbase + ARM_L2PTABLE_BYTES())
+        && ValidMemRange(vbase, vbase + ARM_L2PTABLE_BYTES())
     requires 0 <= index <= ARM_L2PTES()
     ensures var r := ExtractAbsL2PTable(m, vbase, index);
         r.Just? ==> |fromJust(r)| == ARM_L2PTES() - index
@@ -626,7 +561,8 @@ function ExtractAbsL2PTable(m:memstate, vbase:int, index:nat): Maybe<AbsL2PTable
     // stopping condition
     if index == ARM_L2PTES() then Just([]) else
     // extract PTE and check its validity
-    var pte := ExtractAbsL2PTE(MemContents(m, vbase + index * BytesPerWord()));
+    var pte := ExtractAbsL2PTE(
+            MemContents(m, vbase + index * BytesPerWord()));
     if pte.Nothing? then Nothing else
     // extract the rest (recursive step)
     var rest := ExtractAbsL2PTable(m, vbase, index + 1);
@@ -634,26 +570,26 @@ function ExtractAbsL2PTable(m:memstate, vbase:int, index:nat): Maybe<AbsL2PTable
     Just([fromJust(pte)] + fromJust(rest))
 }
 
-function ExtractAbsL2PTE(pte:int): Maybe<Maybe<AbsPTE>>
-    requires isUInt32(pte)
+function ExtractAbsL2PTE(pte:word): Maybe<Maybe<AbsPTE>>
     ensures var r := ExtractAbsL2PTE(pte);
         r.Just? && fromJust(r).Just? ==> WellformedAbsPTE(fromJust(fromJust(r)))
 {
-    var typebits := and32(pte, 0x3);
+    var typebits := BitwiseAnd(pte, 0x3);
     // if the type is zero, it's an invalid entry, which is fine (maps nothing)
     if typebits == 0 then Just(Nothing) else
     // large pages aren't supported
     if typebits == 1 then Nothing else
-    var lowbits := and32(pte, 0xfdfc);
+    var lowbits := BitwiseAnd(pte, 0xfdfc);
     if lowbits != ARM_L2PTE_CONST_BITS() then Nothing else
-    var exec := and32(pte, 1) == 0; // !XN bit
-    var write := and32(pte, 0x200) == 0; // !AP2 bit
+    var exec := BitwiseAnd(pte, 1) == 0; // !XN bit
+    var write := BitwiseAnd(pte, 0x200) == 0; // !AP2 bit
     MaskWithSizeIsAligned(pte, 0x1000);
-    var pagebase := and32(pte, 0xfffff000);
+    var pagebase := BitwiseAnd(pte, 0xfffff000);
+    if !isUInt32(pagebase + PhysBase()) then Nothing else
     Just(Just(AbsPTE(pagebase, write, exec)))
 }
 
-function ARM_L2PTE_CONST_BITS(): int
+function ARM_L2PTE_CONST_BITS(): word
 {
     0x4 /* B */
         + 0x30 /* AP0, AP1 */
@@ -665,52 +601,39 @@ function ARM_L2PTE_CONST_BITS(): int
 //-----------------------------------------------------------------------------
 // Functions for bitwise operations
 //-----------------------------------------------------------------------------
-function xor32(x:int, y:int) : int  
-    requires isUInt32(x) && isUInt32(y);
-    { int(BitwiseXor(uint32(x), uint32(y))) }
 
-function and32(x:int, y:int) : int  
-    requires isUInt32(x) && isUInt32(y);
-    { int(BitwiseAnd(uint32(x), uint32(y))) }
+function {:opaque} BitwiseXor(x:word, y:word): word
+    { (x as bv32 ^ y as bv32) as int }
 
-function or32(x:int, y:int) : int  
-    requires isUInt32(x) && isUInt32(y);
-    { int(BitwiseOr(uint32(x), uint32(y))) }
+function {:opaque} BitwiseAnd(x:word, y:word): word
+    { (x as bv32 & y as bv32) as int }
 
-function not32(x:int) : int  
-    requires isUInt32(x);
-    { int(BitwiseNot(uint32(x))) }
+function {:opaque} BitwiseOr(x:word, y:word): word
+    { (x as bv32 | y as bv32) as int }
 
-function rol32(x:int, amount:int) : int 
-    requires isUInt32(x) && 0 <= amount < 32;
-    { int(RotateLeft(uint32(x), uint32(amount))) }
+function {:opaque} BitwiseNot(x:word): word
+    { !(x as bv32) as int } // is ~ !?
 
-function ror32(x:int, amount:int) : int 
-    requires isUInt32(x) && 0 <= amount < 32;
-    { int(RotateRight(uint32(x), uint32(amount))) }
+function {:opaque} LeftShift(x:word, amount:word): word
+    requires 0 <= amount < 32;
+    { (x as bv32 << amount) as int }
 
-function shl32(x:int, amount:int) : int 
-    requires isUInt32(x) && 0 <= amount < 32;
-    { int(LeftShift(uint32(x), uint32(amount))) }
+function {:opaque} RightShift(x:word, amount:word): word
+    requires 0 <= amount < 32;
+    { (x as bv32 >> amount) as int }
 
-function shr32(x:int, amount:int) : int 
-    requires isUInt32(x) && 0 <= amount < 32;
-    { int(RightShift(uint32(x), uint32(amount))) }
-
-// FIXME! replace this when Dafny gains bitvector support
-lemma {:axiom} MaskWithSizeIsAligned(x:int, s:int)
-    requires isUInt32(x) && isUInt32(s)
+// FIXME! replace this (when we get around to proving it)
+lemma {:axiom} MaskWithSizeIsAligned(x:word, s:word)
     // s must be a power of two. this is a cheesy approximation for that
     requires s == 0x1000 || s == 0x400
-    ensures and32(x, 0x1_0000_0000 - s) % s == 0
+    ensures BitwiseAnd(x, 0x1_0000_0000 - s) % s == 0
 
 //-----------------------------------------------------------------------------
 // Evaluation
 //-----------------------------------------------------------------------------
-function OperandContents(s:state, o:operand): int
+function OperandContents(s:state, o:operand): word
     requires ValidOperand(o)
     requires ValidState(s)
-    ensures  isUInt32(OperandContents(s,o))
 {
     reveal_ValidRegState();
     match o
@@ -720,59 +643,47 @@ function OperandContents(s:state, o:operand): int
         case OLR => s.regs[LR(mode_of_state(s))]
 }
 
-function SpecialOperandContents(s:state, o:operand): int
+function SpecialOperandContents(s:state, o:operand): word
     requires ValidSpecialOperand(s, o)
     requires ValidState(s)
-    ensures  isUInt32(SpecialOperandContents(s,o))
 {
     reveal_ValidSRegState();
     match o
         case OSReg(sr) => s.sregs[sr] 
 }
 
-function MemContents(s:memstate, m:mem): int
+function MemContents(s:memstate, m:mem): word
     requires ValidMemState(s)
-    requires ValidMem(s,m)
-    ensures isUInt32(MemContents(s,m))
+    requires ValidMem(m)
 {
     reveal_ValidMemState();
-    assert m in s.addresses;
-    assert isUInt32(s.addresses[m]);
+    //assert m in s.addresses;
     s.addresses[m]
 }
 
-function GlobalFullContents(s:memstate, g:operand): seq<int>
+function GlobalFullContents(s:memstate, g:operand): seq<word>
     requires ValidMemState(s)
     requires ValidGlobal(g)
-    ensures forall w :: w in GlobalFullContents(s, g) ==> isUInt32(w)
     ensures WordsToBytes(|GlobalFullContents(s, g)|) == SizeOfGlobal(g)
 {
     reveal_ValidMemState();
     s.globals[g]
 }
 
-function GlobalWord(s:memstate, g:operand, offset:int): int
+function GlobalWord(s:memstate, g:operand, offset:word): word
     requires ValidGlobalOffset(g, offset)
     requires ValidMemState(s)
-    ensures isUInt32(GlobalWord(s, g, offset))
 {
     reveal_ValidMemState();
     GlobalFullContents(s, g)[BytesToWords(offset)]
 }
 
-function eval_op(s:state, o:operand): int
-    requires ValidState(s)
-    requires ValidOperand(o)
-    ensures isUInt32(eval_op(s,o))
-    { OperandContents(s,o) }
-
 function takestep(s:state): state
     { s.(steps := s.steps + 1) }
 
-predicate evalUpdate(s:state, o:operand, v:int, r:state)
+predicate evalUpdate(s:state, o:operand, v:word, r:state)
     requires ValidState(s)
-    requires ValidDestinationOperand(o)
-    requires isUInt32(v)
+    requires ValidRegOperand(o)
     ensures evalUpdate(s, o, v, r) ==> ValidState(r)
 {
     reveal_ValidRegState();
@@ -782,12 +693,10 @@ predicate evalUpdate(s:state, o:operand, v:int, r:state)
         case OSP => r == takestep(s).(regs := s.regs[SP(mode_of_state(s)) := v])
 }
 
-
-predicate evalSRegUpdate(s:state, o:operand, v:int, r:state)
+predicate evalSRegUpdate(s:state, o:operand, v:word, r:state)
     requires ValidState(s)
     requires ValidSpecialOperand(s, o)
-    requires isUInt32(v)
-    requires o.sr.cpsr? || o.sr.spsr? ==> ValidModeEncoding(and32(v,0x1f))
+    requires o.sr.cpsr? || o.sr.spsr? ==> ValidModeEncoding(BitwiseAnd(v,0x1f))
     ensures  evalSRegUpdate(s, o, v, r) ==> ValidState(r)
 {
     reveal_ValidSRegState();
@@ -795,20 +704,18 @@ predicate evalSRegUpdate(s:state, o:operand, v:int, r:state)
         sregs := s.sregs[ o.sr := v] )
 }
 
-predicate evalMemUpdate(s:state, m:mem, v:int, r:state)
+predicate evalMemUpdate(s:state, m:mem, v:word, r:state)
     requires ValidState(s)
-    requires ValidMem(s.m, m)
-    requires isUInt32(v)
+    requires ValidMem(m)
     ensures evalMemUpdate(s, m, v, r) ==> ValidState(r)
 {
     reveal_ValidMemState();
     r == takestep(s).(m := s.m.(addresses := s.m.addresses[m := v]))
 }
 
-predicate evalGlobalUpdate(s:state, g:operand, offset:nat, v:int, r:state)
+predicate evalGlobalUpdate(s:state, g:operand, offset:word, v:word, r:state)
     requires ValidState(s)
     requires ValidGlobalOffset(g, offset)
-    requires isUInt32(v)
     ensures evalGlobalUpdate(s, g, offset, v, r) ==> ValidState(r) && GlobalWord(r.m, g, offset) == v
 {
     reveal_ValidMemState();
@@ -818,7 +725,7 @@ predicate evalGlobalUpdate(s:state, g:operand, offset:nat, v:int, r:state)
     r == takestep(s).(m := s.m.(globals := s.m.globals[g := newval]))
 }
 
-function evalCmp(c:ocmp, i1:int, i2:int):bool
+function evalCmp(c:ocmp, i1:word, i2:word):bool
 {
   match c
     case OEq => i1 == i2
@@ -853,10 +760,9 @@ predicate ValidModeChange'(s:state, m:mode)
     priv_of_state(s) == PL1 && !(m == Monitor && world_of_state(s) != Secure)
 }
 
-predicate ValidModeChange(s:state, v:int)
-    requires isUInt32(v)
+predicate ValidModeChange(s:state, v:word)
 {
-    var enc := and32(v,0x1f);
+    var enc := psr_mask_mode(v);
     ValidModeEncoding(enc) && ValidModeChange'(s, decode_mode(enc))
 }
 
@@ -865,54 +771,53 @@ predicate ValidInstruction(s:state, ins:ins)
     // reveal_ValidConfig();
     ValidState(s) && match ins
         case ADD(dest, src1, src2) => ValidOperand(src1) &&
-            ValidOperand(src2) && ValidDestinationOperand(dest) &&
-            isUInt32(eval_op(s,src1) + eval_op(s,src2))
+            ValidOperand(src2) && ValidRegOperand(dest) &&
+            isUInt32(OperandContents(s,src1) + OperandContents(s,src2))
         case SUB(dest, src1, src2) => ValidOperand(src1) &&
-            ValidOperand(src2) && ValidDestinationOperand(dest) &&
-            isUInt32(eval_op(s,src1) - eval_op(s,src2))
+            ValidOperand(src2) && ValidRegOperand(dest) &&
+            isUInt32(OperandContents(s,src1) - OperandContents(s,src2))
         case MUL(dest,src1,src2) => ValidRegOperand(src1) &&
-            ValidRegOperand(src2) && ValidDestinationOperand(dest) &&
-            isUInt32(eval_op(s,src1) * eval_op(s,src2))
+            ValidRegOperand(src2) && ValidRegOperand(dest) &&
+            isUInt32(OperandContents(s,src1) * OperandContents(s,src2))
         case UDIV(dest,src1,src2) => ValidOperand(src1) &&
-            ValidOperand(src2) && ValidDestinationOperand(dest) &&
-            (eval_op(s,src2) > 0) && isUInt32(eval_op(s,src1) / eval_op(s,src2))
+            ValidOperand(src2) && ValidRegOperand(dest) &&
+            (OperandContents(s,src2) > 0) &&
+            isUInt32(OperandContents(s,src1) / OperandContents(s,src2))
         case AND(dest, src1, src2) => ValidOperand(src1) &&
-            ValidOperand(src2) && ValidDestinationOperand(dest)
+            ValidOperand(src2) && ValidRegOperand(dest)
         case ORR(dest, src1, src2) => ValidOperand(src1) &&
-            ValidOperand(src2) && ValidDestinationOperand(dest)
+            ValidOperand(src2) && ValidRegOperand(dest)
         case EOR(dest, src1, src2) => ValidOperand(src1) &&
-            ValidOperand(src2) && ValidDestinationOperand(dest)
-        case ROR(dest, src1, src2) => ValidOperand(src1) &&
-            ValidShiftOperand(s, src2) && ValidDestinationOperand(dest)
+            ValidOperand(src2) && ValidRegOperand(dest)
         case LSL(dest, src1, src2) => ValidOperand(src1) &&
-            ValidShiftOperand(s, src2) && ValidDestinationOperand(dest)
+            ValidShiftOperand(s, src2) && ValidRegOperand(dest)
         case LSR(dest, src1, src2) => ValidOperand(src1) &&
-            ValidShiftOperand(s, src2) && ValidDestinationOperand(dest)
+            ValidShiftOperand(s, src2) && ValidRegOperand(dest)
         case MVN(dest, src) => ValidOperand(src) &&
-            ValidDestinationOperand(dest)
+            ValidRegOperand(dest)
         case LDR(rd, base, ofs) => 
-            ValidDestinationOperand(rd) &&
+            ValidRegOperand(rd) &&
             ValidOperand(base) && ValidOperand(ofs) &&
             WordAligned(OperandContents(s, base) + OperandContents(s, ofs)) &&
-            ValidMem(s.m, OperandContents(s, base) + OperandContents(s, ofs))
+            ValidMem(OperandContents(s, base) + OperandContents(s, ofs))
         case LDR_global(rd, global, base, ofs) => 
-            ValidDestinationOperand(rd) &&
+            ValidRegOperand(rd) &&
             ValidOperand(base) && ValidOperand(ofs) &&
             AddressOfGlobal(global) == OperandContents(s, base) &&
             ValidGlobalOffset(global, OperandContents(s, ofs))
         case LDR_reloc(rd, global) => 
-            ValidDestinationOperand(rd) && ValidGlobal(global)
+            ValidRegOperand(rd) && ValidGlobal(global)
         case STR(rd, base, ofs) =>
             ValidRegOperand(rd) &&
             ValidOperand(ofs) && ValidOperand(base) &&
             WordAligned(OperandContents(s, base) + OperandContents(s, ofs)) &&
-            ValidMem(s.m, OperandContents(s, base) + OperandContents(s, ofs))
+            ValidMem(OperandContents(s, base) + OperandContents(s, ofs))
         case STR_global(rd, global, base, ofs) => 
             ValidRegOperand(rd) &&
             ValidOperand(base) && ValidOperand(ofs) &&
             AddressOfGlobal(global) == OperandContents(s, base) &&
             ValidGlobalOffset(global, OperandContents(s, ofs))
-        case MOV(dst, src) => ValidDestinationOperand(dst) &&
+        case MOV(dst, src) => ValidRegOperand(dst) &&
             ValidOperand(src)
         case MRS(dst, src) =>
             ValidSpecialOperand(s, src) &&
@@ -953,28 +858,24 @@ predicate evalIns(ins:ins, s:state, r:state)
             ((OperandContents(s, src1) / OperandContents(s, src2))),
             r)
         case AND(dst, src1, src2) => evalUpdate(s, dst,
-            and32(eval_op(s, src1), eval_op(s, src2)),
+            BitwiseAnd(OperandContents(s, src1), OperandContents(s, src2)),
             r)
         case ORR(dst, src1, src2) => evalUpdate(s, dst,
-            or32(eval_op(s, src1), eval_op(s, src2)),
+            BitwiseOr(OperandContents(s, src1), OperandContents(s, src2)),
             r)
         case EOR(dst, src1, src2) => evalUpdate(s, dst,
-            xor32(eval_op(s, src1), eval_op(s, src2)),
+            BitwiseXor(OperandContents(s, src1), OperandContents(s, src2)),
             r)
-        case ROR(dst, src1, src2) => if !(src2.OConst? && 0 <= src2.n <32) then !r.ok
-            else evalUpdate(s, dst,
-                ror32(eval_op(s, src1), eval_op(s, src2)),
-                r)
         case LSL(dst, src1, src2) => if !(src2.OConst? && 0 <= src2.n <32) then !r.ok 
             else evalUpdate(s, dst,
-                shl32(eval_op(s, src1), eval_op(s, src2)),
+                LeftShift(OperandContents(s, src1), OperandContents(s, src2)),
                 r)
         case LSR(dst, src1, src2) => if !(src2.OConst? && 0 <= src2.n <32) then !r.ok
             else evalUpdate(s, dst,
-                shr32(eval_op(s, src1), eval_op(s, src2)),
+                RightShift(OperandContents(s, src1), OperandContents(s, src2)),
                 r)
         case MVN(dst, src) => evalUpdate(s, dst,
-            not32(eval_op(s, src)), r)
+            BitwiseNot(OperandContents(s, src)), r)
         case LDR(rd, base, ofs) => 
             evalUpdate(s, rd, MemContents(s.m, OperandContents(s, base) +
                 OperandContents(s, ofs)), r)
@@ -997,28 +898,16 @@ predicate evalIns(ins:ins, s:state, r:state)
         case MOVS_PCLR_TO_USERMODE_AND_CONTINUE => evalMOVSPCLRUC(s, r)
 }
 
-/*
-predicate AlwaysInvariant(s:state, s':state)
-{
-    // valid state is maintained
-    ValidState(s) && ValidState(s')
-    // mem validity never changes
-    && (forall m:mem :: m in s.m.addresses <==> m in s'.m.addresses)
-}
-*/
-
 predicate evalMOVSPCLRUC(s:state, r:state)
     requires ValidState(s)
-    ensures  evalMOVSPCLRUC(s, r) ==> ValidState(r)
-    ensures  evalMOVSPCLRUC(s, r) ==> r.ok
+    ensures  evalMOVSPCLRUC(s, r) ==> ValidState(r) && r.ok
 {
-            exists ex, s2, s3, s4
-                :: ValidState(s2) && ValidState(s3) && ValidState(s4)
-                && evalEnterUserspace(s, s2)
-                && evalUserspaceExecution(s2, s3)
-                && evalExceptionTaken(s3, ex, s4)
-                && ApplicationUsermodeContinuationInvariant(s4, r)
-                && r.ok
+    exists ex, s2, s3, s4 :: ValidState(s2) && ValidState(s3) && ValidState(s4)
+        && evalEnterUserspace(s, s2)
+        && evalUserspaceExecution(s2, s3)
+        && evalExceptionTaken(s3, ex, s4)
+        && ApplicationUsermodeContinuationInvariant(s4, r)
+        && r.ok
 }
 
 predicate evalBlock(block:codes, s:state, r:state)
